src/ListSupport.v
@@ -1,0 +1,43 @@
+Require Import Common List.
+
+Set Implicit Arguments.
+
+Lemma tl_app:
+  forall {A} (l1 l2: list A),
+    l1 <> nil -> tl (l1 ++ l2) = (tl l1) ++ l2.
+Proof.
+  destruct l1; intuition idtac.
+Qed.
+
+Lemma cons_app:
+  forall {A} (a: A) (l: list A),
+    a :: l = (a :: nil) ++ l.
+Proof.
+  reflexivity.
+Qed.
+
+Lemma Forall_app:
+  forall {A} (l1 l2: list A) P,
+    Forall P l1 -> Forall P l2 -> Forall P (l1 ++ l2).
+Proof.
+  induction l1; simpl; intros; auto.
+  inv H; constructor; auto.
+Qed.
+
+Lemma Forall_remove:
+  forall {A} dec P (a: A) (l: list A),
+    Forall P l -> Forall P (remove dec a l).
+Proof.
+  induction l; simpl; intros; auto.
+  inv H; destruct (dec a a0); auto.
+Qed.
+
+Lemma Forall_filter:
+  forall {A} P f (l: list A),
+    Forall P l -> Forall P (filter f l).
+Proof.
+  induction l; simpl; intros; auto.
+  inv H.
+  destruct (f a); auto.
+Qed.
+
