src/SingleValue.v
@@ -357,6 +357,7 @@ Section Sim.
           { left; reflexivity. }
           { simpl; auto. }
           { simpl; reflexivity. }
+          { admit. }
         * admit.
           
       + admit.
